%!TEX root = main.tex

\section{RK2 Ralston}
RK2 is a popular $2$-nd order method. The scheme for
solving $\dot{x}(t) = g(x(t))$ is defined as follows
\begin{align*}
k_{1} &= g(x_{k}) \\
k_{2} &= g(x_{k} + \eta \frac{3}{4} k_1) \\
x_{k + 1} &= x_{k} + \frac{\eta}{4} \big( k_{1} + 3 k_{2} \big)
\end{align*}
Now, if we have optimize a function, $f$, then the
RK2-Ralston Optimization Scheme is defined as follows:
\begin{align*}
  x_{k + 1} = x_{k} - \frac{\eta}{4} (\nabla f(x)
  + 3\nabla f(x - \frac{2}{3}\eta \nabla f(x)))
\end{align*}

\subsection{Strongly Convex}
\begin{theorem}\label{rk2 ralston stongly convex}
  Let $f$ be $\beta$-smooth and $\alpha$-Strongly
  Convex function. Then let $\eta = \frac{2}{\alpha + \beta}$.
Then RK-2 Ralston  satisfies:
\begin{align*}
  f(x_{k}) - f(x^{*}) \leq \frac{\beta}{2}\exp(-\frac{4 k}{\kappa + 1})
  \norm{x_{1} - x^{*}}_{2}^{2}
\end{align*}
where $\kappa = \frac{\beta}{\alpha}$ is the condition number.
\end{theorem}
\begin{proof}
  Define $r_k = \norm{x_{k} - x^{*}}$ and $F(x) =
  \nabla f(x) - 3\nabla f(x - \frac{2}{3}\eta \nabla f(x)) = k_{1} + 3k_{2}$,
\begin{align*}
\norm{x_{k + 1} - x^{*}}^{2} &= \norm{x_{k} - x^{*} - \frac{\eta}{4} F(x_k) }^{2} \\
                             &= \norm{x_{k} - x^{*}}^{2}
                               + \frac{\eta^{2}}{16}\norm{F(x_k)}^{2}
                               - \frac{\eta}{2}(x_{k} - x^{*})^{T} F(x_{k}) \\ \label{sc_rk2_ralston}
                             &= \norm{x_{k} - x^{*}}^{2}
                               + \frac{\eta^{2}}{16}\norm{k_{1}
                               + 3 k_{2}}^{2} - \frac{\eta}{2}(x_{k} - x^{*})^{T} F(x_{k}) \\
&= \norm{x_{k} - x^{*}}^{2} + \frac{\eta^{2}}{16}( \norm{k_{1}}^{2} + 9 \norm{k_{2}}^{2} + 6 k_{1}^{T} k_{2}) - \frac{\eta}{2}(x_{k} - x^{*})^{T} k_{1} - \frac{3\eta}{2}(x_{k} - x^{*})^{T}  k_{2} \\
&= \norm{x_{k} - x^{*}}^{2} + \frac{\eta^{2}}{16}( \norm{k_{1}}^{2} + 9 \norm{k_{2}}^{2} + 6 k_{1}^{T} k_{2}) - \frac{\eta}{2}(x_{k} - x^{*})^{T} k_{1} \\
& \qquad \qquad - \frac{3\eta}{2}(x_{k} - \frac{2 \eta}{3}k_{1} - x^{*})^{T}  k_{2} - \eta^{2} k_{1}^{T} k_{2} \\
& \leq \norm{x_{k} - x^{*}}^{2} + \frac{\eta^{2}}{16}( \norm{k_{1}}^{2} + 9 \norm{k_{2}}^{2}) - \frac{\eta}{2}(x_{k} - x^{*})^{T} k_{1} - \frac{3\eta}{2}(x_{k} - \frac{2 \eta}{3}k_{1} - x^{*})^{T}  k_{2}
\end{align*}
Then again by equation \eqref{coercivity}, then the above equation becomes,
\begin{align*}
r_{k + 1}^{2} & \leq r_{k}^{2} + + \frac{\eta^{2}}{16}( \norm{k_{1}}^{2} + 9 \norm{k_{2}}^{2}) - \frac{\eta}{2}(x_{k} - x^{*})^{T} k_{1} - \frac{3\eta}{2}(x_{k} - \frac{2 \eta}{3}k_{1} - x^{*})^{T}  k_{2}\\
& \leq r_{k}^{2} + \frac{\eta}{4}(\eta - \frac{2}{\alpha + \beta}) \bigg(\norm{k_{1}}^{2} + 3\norm{k_{2}}^{2} \bigg) - \frac{\eta}{2}\frac{\alpha \beta}{\alpha + \beta} \bigg(r_{k}^{2} + 3\norm{x_{k} - \frac{2 \eta}{3} k_{1} - x^{*}}^{2}\bigg)  \\
&= r_{k}^{2} - \frac{\eta}{2}\frac{\alpha \beta}{\alpha + \beta} \bigg(r_{k}^{2} + 3\norm{x_{k} - \frac{2 \eta}{3} k_{1} - x^{*}}^{2}\bigg) \\
&= r_{k}^{2} - \frac{\eta}{2}\frac{\alpha \beta}{\alpha + \beta} \bigg( r_{k}^{2} + 3 r_{k}^{2} + \frac{4 \eta^{2}}{3} \norm{\nabla f(x_k)}^{2} - 4 \eta (x_{k} - x^{*})^{T} \nabla f(x_{k}) \bigg) \\
&=  \bigg( 1 -  \frac{2 \eta \alpha \beta}{\alpha + \beta} \bigg) r_{k}^{2} - \frac{\eta}{2}\frac{\alpha \beta}{\alpha + \beta} \bigg( \frac{4 \eta^{2}}{3} \norm{\nabla f(x_k)}^{2} - 4 \eta (x_{k} - x^{*})^{T} \nabla f(x_{k}) \bigg) \\
& \leq \bigg(\frac{\kappa - 1}{\kappa + 1}\bigg)^{2} r_{k}^{2} %- 2 \eta^{2} \frac{\alpha \beta}{\alpha + \beta} \bigg( \frac{ \eta}{3} \norm{\nabla f(x_k)}^{2} -  (x_{k} - x^{*})^{T} \nabla f(x_{k}) \bigg)
\end{align*}
% Now, as $f$ is $\alpha$-Strongly convex and $\beta$-Smooth, we can show that
% \begin{align*}
% &(\nabla f(x) - \nabla f(y))^{T} (x - y)  \leq \frac{1}{\alpha}\norm{\nabla f(x) - \nabla f(y)}^{2} \\
% & \text{Use this along with \eqref{coercivity}}
% \end{align*}


\end{proof}


\subsection{Convex}
\begin{theorem}\label{rk2 ralston convex}
Let $f: \mathbb{R}^{n} \rightarrow \mathbb{R}$ be convex and $\beta$-smooth, then RK2-Ralston with $\eta = \frac{2}{\beta}$ satisfies the following:
\begin{align}
f(x_{k}) - f(x^{*}) \leq  \frac{4}{3} \frac{\norm{x_{1} - x^{*}}^{2}}{k - 1}
\end{align}
\end{theorem}

\begin{lemma} \label{lemma_2}
Let $f: \mathbb{R}^{n} \rightarrow \mathbb{R}$ be convex and $\beta$-smooth, then RK2-Ralston satisfies the following:
\begin{align*}
f(x_{k + 1}) \leq f(x_{k}) - \frac{3}{4 \beta ( k + 1)} \norm{\nabla f(x_k)}^{2}
\end{align*}
\end{lemma}

% \begin{proof}\ref{lemma_2}
% As done in the previous lemma, define $\Delta x = \nabla f(x) + 3\nabla f(x - \frac{2}{3}\eta \nabla f(x))$, then note that
% \begin{align*}
% f(x_{k + 1}) - f(x_{k}) &\leq - \frac{\eta}{4}\nabla f(x_{k})^{T} \Delta x_{k} + \frac{\eta^{2} \beta}{32} \norm{\Delta x_{k}}^{2} \\
% &= - \frac{\eta}{4}\nabla f(x_{k})^{T}( k_{1} + 3 k_{2} ) + \frac{\eta^{2} \beta}{32} \norm{ k_{1} + 3 k_{2} }^{2} \\
% &= - \frac{\eta}{4} ( \norm{k_{1}}^{2} + 3 k_{1}^{T} k_{2} ) + \frac{\eta^{2} \beta}{32} ( 2 \norm{k_{1}}^{2} + 18 \norm{k_{2}}^{2} ) \\
% &= - \frac{\eta}{4} \norm{k_{1}}^{2} \bigg( 1 - \frac{\eta \beta}{4} \bigg)
%  - \frac{3 \eta}{4} k_{1}^{T} k_{2} + \frac{9 \eta^{2} \beta}{16}\norm{k_{2}^{2}}
% \end{align*}
% Now, note that
% \begin{align*}
% & k_{1}^{T} k_{2}  \sim = \norm{k_{1}}^{2} - \eta \\
% \norm{k_{2}}^{2} &= \norm{k_{1}}^{2} + \frac{4 \eta^{2}}{9} \norm{ \nabla^{2} f(x) k_{1}} -  \frac{4 \eta}{3} k_{1}^{T} \nabla^{2} f(x) k_{1}
% \end{align*}

% \end{proof}

\begin{proof}(Lemma \ref{lemma_2})
Let $\Delta x =  \frac{1}{2\beta}(k_1 + 3k_2)$, where $\eta = \frac{2}{\beta}$ then note that
\begin{equation}
\begin{aligned}\label{ineq0}
f(x - \Delta x) - f(x) &\leq \nabla f(x)^T (x - \Delta x - x) + \frac{\beta}{2} || x - x - \Delta x ||^2 \\
&= -  \nabla f(x)^T ( \Delta x) + \frac{1}{16 \beta} || \Delta x ||^2 \\
&= -\frac{1}{2 \beta} \nabla  f(x)^T ( k_1 + 3k_2) + \frac{1}{16 \beta} || \Delta x ||^2 \\
&= -\frac{1}{2\beta}\nabla f(x)^T k_1 - \frac{3}{2\beta}\nabla f(x)^T k_2 + \frac{1}{16 \beta} || k_1 ||_2^2 + \frac{9}{16 \beta} || k_2 ||^2_2 + \frac{6}{16\beta}\left\langle k_1, k_2 \right\rangle \\
&= -\frac{1}{2\beta}\nabla f(x)^T k_1 +  \frac{1}{16 \beta} || k_1 ||_2^2 -  \frac{3}{2\beta}\nabla f(x)^T k_2 +  \frac{9}{16 \beta} || k_2 ||^2_2  + \frac{6}{16\beta}k_1^{T} k_2 \\
&= -\frac{7}{16 \beta}|| k_1 ||_2^2 -\frac{1}{16 \beta}k_2^T(24 \nabla f(x) - 9 k_2) + \frac{6}{16\beta}k_1^{T} k_2 \\
&= -\frac{7}{16 \beta}|| k_1 ||_2^2 - \frac{24}{16 \beta}k_2^Tk_1 + \frac{6}{16 \beta}k_1^{T} k_2 + \frac{9}{16\beta}|| k_2 ||_2^2 \\
&= -\frac{7}{16 \beta}|| k_1 ||_2^2 - \frac{18}{16 \beta} k_1^{T} k_2 + \frac{9}{16 \beta}|| k_2 ||_2^2
\end{aligned}
\end{equation}

Now, using a Taylor Series approximation for $\nabla f \big( x -  \frac{2\eta}{3}k_1 \big)$, we get that,
\begin{equation}
\begin{aligned}\label{ineq1}
\nabla f \big( x - \frac{2\eta}{3}k_1 \big) &= \nabla f(x) - \frac{2\eta}{3} \nabla^2 f(x) \nabla f(x) + \mathcal{O}( |\frac{2\eta}{3} |^2 ) \\
\implies  k_2^Tk_1 &= \nabla f \big( x - \frac{2\eta}{3}k_1 \big)^T\nabla f(x) \\
 &= \nabla f \big( x - \frac{2\eta}{3}\nabla f(x) \big)^T \nabla f(x) \\
&= || \nabla f(x) ||_2^2 - \frac{2\eta}{3} \nabla f(x)^T \nabla^2 f(x) \nabla f(x)
\end{aligned}
\end{equation}
And, using \eqref{ineq1},
\begin{equation}
\begin{aligned} \label{ineq2}
|| k_2 ||_2^2 &= ||  \nabla f(x) - \frac{2\eta}{3} \nabla^2 f(x) \nabla f(x)  ||_2^2   \\
&= || \nabla f(x)||_2^2 + \frac{4\eta}{9}||\nabla^2 f(x) \nabla f(x)  ||_2^2 - \frac{4\eta}{3} \nabla f(x)^T \nabla^2 f(x) \nabla f(x)
\end{aligned}
\end{equation}
Hence, using \eqref{ineq1} and \eqref{ineq2}
\begin{align*}
f(x - \Delta x) - f(x) & \leq  -\frac{7}{16 \beta}|| k_1 ||_2^2 - \frac{18}{16 \beta}  k_1^{T} k_2  + \frac{9}{16 \beta}|| k_2 ||_2^2 \\
&= -\frac{7}{16 \beta}|| \nabla f(x) ||_2^2 -  \frac{18}{16 \beta} || \nabla f(x) ||_2^2 + \frac{12}{16 \beta^2} \nabla f(x)^T \nabla^2 f(x) \nabla f(x) \\
&+  \frac{9}{16\beta}( || \nabla f(x)||_2^2 + \frac{4}{9\beta}||\nabla^2 f(x) \nabla f(x)  ||_2^2 - \frac{4}{3\beta} \nabla f(x)^T \nabla^2 f(x) \nabla f(x) )  \\
&= -\frac{16}{16 \beta}|| \nabla f(x)||_2^2 + \frac{1}{4 \beta^2}||\nabla^2 f(x) \nabla f(x)  ||_2^2 \\
&= -\frac{1}{\beta} || \nabla f(x)||_2^2 + \frac{1}{4 \beta^2}||\nabla^2 f(x) \nabla f(x)  ||_2^2 \\
\end{align*}
Using the lipschitz property of the Hessian of $f$, $||\nabla^2 f(x) u - \nabla^2 f(x) v||_2^2 \leq \beta || u-v ||_2^2 $, we get that,
\begin{equation}
\begin{aligned}
f(x - \Delta x) - f(x) & \leq -\frac{1}{\beta} || \nabla f(x)||_2^2 + \frac{1}{4\beta^2}||\nabla^2 f(x) \nabla f(x)  ||_2^2 \\
& \leq -\frac{4}{4\beta}|| \nabla f(x) ||_2^2 + \frac{\beta}{4 \beta^2}|| \nabla f(x) ||_2^2 \\
& = -\big( \frac{4}{4\beta} - \frac{\beta}{8\beta^2}   \big)  || \nabla f(x) ||_2^2  \\
&= -\frac{3}{4\beta} || \nabla f(x) ||_2^2
\end{aligned}
\end{equation}
\end{proof}

\begin{proof}(Theorem \ref{rk2 ralston convex})
Using Lemma 1, we have $f(x_{t+1}) - f(x_{t}) \leq -\frac{3}{4\beta}|| \nabla f(x_{t}) ||_2^2 $. Now, let $\delta_t = f(x_t) - f(x^*)$, then note that:
\begin{align*}
\delta_{t+1} \leq \delta_t - \frac{3}{4\beta}|| \nabla f(x) ||_2^2
\end{align*}
Now, by convexity of $f(x)$ we have:
\begin{align}
\delta_t &\leq \nabla f(x_t)^T (x_t - x^*) \\
 &\leq || x_t - x^* ||_2 * || \nabla f(x_t) ||_2 \\
\frac{1}{|| x_t - x^* || }\delta_t^2 & \leq  || \nabla f(x_t) ||_2^2
\end{align}

Now, note that $|| x_t - x^*||_2^2$ is decreasing, using the following inequality
\begin{align*}
\big( \nabla f(x) - \nabla f(y)  \big)^T(x-y)  \geq \frac{1}{\beta} || \nabla f(x) - \nabla f(y) ||_2^2
\end{align*}
Using the above and the fact that $\nabla f(x^*) = 0$,
\begin{align*}
|| x_{t+1} - x^* ||_2^2 &= || x_t - \Delta x_t - x^* ||_2^2 \\
&= || x_t - x^* ||_2^2 + || \Delta x_t ||_2^2 - 2 \Delta x_t^T(x_t - x^*) \\
&= || x_t - x^* ||_2^2 - \frac{1}{\beta}(k_1 + 3k_2)^T (x_t - x^*) + \frac{1}{4 \beta^2}|| k_1 + 3k_2 ||_2^2 \\
&= || x_t - x^* ||_2^2 - \frac{1}{ \beta}k_1^T (x_t - x^*) + \frac{1}{4 \beta^2}|| k_1 ||_2^2  \\
& \quad \quad \quad - \frac{3}{\beta}k_2^T (x_t - x^*) + \frac{9}{4 \beta^2}|| k_2 ||_2^2 + \frac{6}{4 \beta^2} k_1 ^T k_2 \\
&= || x_t - x^* ||_2^2 - \frac{4}{4 \beta^2}||k_1 ||_2^2 + \frac{1}{4 \beta^2}|| k_1 ||_2^2  \\
& \quad \quad \quad - \frac{12}{4 \beta^2}|k_2||_2^2 + \frac{9}{4 \beta^2}|| k_2 ||_2^2 + \frac{6}{4 \beta^2} k_1 ^T k_2 \\
&= || x_t - x^* ||_2^2 - \frac{3}{4 \beta^2}||k_1||_2^2 - \frac{3}{4 \beta^2}||k_2||_2^2 + \frac{6}{4 \beta^2} k_1 ^T k_2 \\
&= || x_t - x^* ||_2^2 -  \frac{3}{4 \beta^2}|| k_1 - k_2||_2^2  \\
& \leq || x_t - x^* ||_2^2
\end{align*}
We will show that,
\begin{align}
\delta_{t+1} \leq \delta_t - \frac{3}{4 \beta || x_1 - x^* ||_2^2} \delta_t^2
\end{align}
Now, let $\omega = \frac{3}{4 \beta   || x_1 - x^* ||_2^2}$, %then note that: (Proof in Bubek page - 269)
\begin{align*}
& \frac{1}{\delta_t} \geq \omega (t-1) \\
\implies & f(x_t) - f(x^*) \leq \frac{4}{3 \beta} \frac{ || x_1 - x^* ||_2^2}{t-1} \xrightarrow{t \to \infty} 0
\end{align*}
\end{proof}


% \subsection{Stochastic -  Strongly Convex}


%%% Local Variables:
%%% mode: latex
%%% TeX-master: "main"
%%% End:
