%!TEX root=./optim_report.tex
\subsection{RK2 Heun Proof}
\begin{proof}(Lemma 2)
% Let $\Delta x = \frac{1}{2\beta}(k_1 + k_2) $, then using Taylor Series approximation we get that:
% \begin{equation}
% \begin{aligned}
% f(x - \Delta x) - f(x) &\leq \nabla f(x)^T ( - \Delta x) + \frac{\beta}{2}|| \Delta x||_2^2 \\
% & = - \frac{1}{2\beta}\nabla f(x)^T (k_1 + k_2) + \frac{1}{8\beta}||k_1 + k_2 ||_2^2 \\
% & = - \frac{1}{2\beta}\nabla ||f(x)||_2^2 - \frac{1}{2\beta}\nabla f(x)^T k_2 + \frac{1}{8\beta}||\nabla f(x)||_2^2 + \frac{1}{8\beta}||k_2||_2^2 + \frac{1}{2\beta}k_1^T k_2 \\
% & = -\frac{3}{8\beta}||\nabla f(x)||_2^2 + \frac{1}{8\beta}||k_2||_2^2 \\
% & = -\frac{3}{8\beta}||\nabla f(x)||_2^2 + \frac{1}{8\beta}||\nabla f(x)||_2^2 + \frac{1}{8\beta^2}||\nabla^2 f(x) \nabla f(x)||_2^2 \\
% & \leq - \frac{1}{8\beta}|| \nabla f(x)||_2^2
% \end{aligned}
% \end{equation}
Let $\Delta x = \frac{1}{\beta}(k_1 + k_2) $, then using Taylor Series approximation we get that:

\begin{equation}
\begin{aligned}
f(x - \Delta x) - f(x) &\leq \nabla f(x)^T ( - \Delta x) + \frac{\beta}{2}|| \Delta x||_2^2 \\
& = - \frac{1}{\beta}\nabla f(x)^T (k_1 + k_2) + \frac{1}{2\beta}||k_1 + k_2 ||_2^2 \\
& = - \frac{1}{\beta}\nabla ||f(x)||_2^2 - \frac{1}{\beta}\nabla f(x)^T k_2 + \frac{1}{2\beta}||\nabla f(x)||_2^2 + \frac{1}{2\beta}||k_2||_2^2 + \frac{1}{\beta}k_1^T k_2 \\
& \leq -\frac{1}{2\beta}||\nabla f(x)||_2^2 + \frac{1}{\beta}||k_2||_2^2 \\
& = -\frac{1}{2\beta}||\nabla f(x)||_2^2 + \frac{1}{\beta}||\nabla f(x)||_2^2 + \frac{4}{\beta^2}||\nabla^2 f(x) \nabla f(x)||_2^2 \\
& \leq - \frac{3}{2\beta}|| \nabla f(x)||_2^2
\end{aligned}
\end{equation}

\end{proof}

\subsection{Order Of Convergence}
Here we show that RK2-Heun and also RK2-ralston both achieve a linear rate of convergence.
\\
\\
Let $r_k = || x_k - x^* ||$, the note that
\begin{equation}
\begin{aligned}
x_{k+1} - x^* &= x_{k} - x^* - \frac{1}{2\beta} \big( \nabla f(x_k) + \nabla f(x_k - \frac{1}{\beta} \nabla f(x_k))  \big)\\
 &= x_{k} - x^* - \frac{1}{2\beta} \big( \nabla f(x_k) - \nabla f(x^*) \big) - \frac{1}{2\beta} \big( \nabla f(x_k - \frac{1}{\beta} \nabla f(x_k)) - \nabla f(x^*) \big) \\
 &= x_{k} - x^* - \frac{1}{2\beta} \int_0^1 \nabla^2 f(x^* + t(x_k - x^*)(x_k - x^*)dt \\
& \quad \quad \quad \quad - \frac{1}{2\beta} \int_0^1 \nabla^2 f(x^* + t(x_k - x^* - \frac{1}{\beta} \nabla f(x_k) )(x_k - x^* - \frac{1}{\beta} \nabla f(x_k))dt \\
\end{aligned}
\end{equation}
Now, let $z_k = x_k - x^*$, then note that
\begin{equation}
\begin{aligned}
y_{k+1} &= y_k - \frac{1}{2\beta} \int_0^1 \nabla^2 f(x^* + ty_k)y_kdt - \frac{1}{2\beta} \int_0^1 \nabla^2 f(x^* + t(y_k - \frac{1}{\beta} \nabla f(x_k))(y_k - \frac{1}{\beta} \nabla f(x_k))dt \\
&= \big(I -  \frac{1}{2\beta} \int_0^1 \nabla^2 f(x^* + ty_k) + \nabla^2 f(x^* + t(y_k - \frac{1}{\beta} \nabla f(x_k)) dt  \big) y_k \\
& \quad \quad \quad \quad  + \frac{1}{2\beta} \int_0^1 \nabla^2 f(x^* + t(y_k - \frac{1}{\beta} \nabla f(x_k)) \frac{1}{\beta} \nabla f(x_k) dt \\
&= \big(I -  \frac{1}{2\beta} \int_0^1 \nabla^2 f(x^* + ty_k) + \nabla^2 f(x^* + t(y_k - \frac{1}{\beta} \nabla f(x_k)) dt  \big) y_k \\
& \quad \quad \quad \quad  + \frac{1}{2\beta^2} \int_0^1 \nabla^2 f(x^* + t(y_k - \frac{1}{\beta} \nabla f(x_k)) ( \nabla f(x_k)  - \nabla f(x^*) )dt
\end{aligned}
\end{equation}
Now, define the following operators:
\begin{equation}
\begin{aligned}
H_k &=  \big(I -  \frac{1}{2\beta} \int_0^1 \nabla^2 f(x^* + ty_k) + \nabla^2 f(x^* + t(y_k - \frac{1}{\beta} \nabla f(x_k)) dt  \big) \\
G_k &= \frac{1}{2\beta^2} \int_0^1 \nabla^2 f(x^* + t(y_k - \frac{1}{\beta} \nabla f(x_k)) dt
\end{aligned}
\end{equation}
Then note that as $f \in C_{\beta}^{2,2}( \mathbb{R}^n) \cap  C_{\beta}^{2,1}( \mathbb{R}^n) $,
\begin{align} \label{ineq4}
|| \nabla^2 f(x) || \leq \beta \\
|| \nabla f(x) || = || \nabla f(x) - \nabla f(x^*) ||& \leq  \beta || x - x^* ||  \label{ineq5}
\end{align}
Now, using \eqref{ineq4} and \eqref{ineq5}, we have:
\begin{equation}
\begin{aligned}
|| G_k ( \nabla f(x_k)  - \nabla f(x^*) ) || &\leq || G_k ||* ||  \nabla f(x_k)  - \nabla f(x^* )|| \\
& \leq  \frac{1}{2\beta^2} \int_0^1 || \nabla^2 f(x^* + t(y_k - \frac{1}{\beta} \nabla f(x_k)) || * ||  \nabla f(x_k)  - \nabla f(x^*) ||  dt \\
& \leq \frac{1}{2 \beta^2} \int_{0}^1 \beta^2 || x_k -  x^* || dt =\frac{1}{2} || x_k - x^* ||  = \frac{1}{2} r_k
\end{aligned}
\end{equation}
And now we obtain a similar bound for $H_k$,

\begin{equation}
\begin{aligned}
 H_k &= I -  \frac{1}{2\beta} \int_0^1 \nabla^2 f(x^* + ty_k) + \nabla^2 f(x^* + t(y_k - \frac{1}{\beta} \nabla f(x_k)) dt  \\
 & \leq I + \frac{1}{\beta} \nabla^2 f(x^*) - \frac{1}{2 \beta}   \int_0^1 \nabla^2 f(x^* + ty_k) -  \nabla^2 f(x^*) + \nabla^2 f(x^* + t(y_k - \frac{1}{\beta} \nabla f(x_k)) -  \nabla^2 f(x^*) dt \\
 ||H_k ||&  \leq || I + \frac{1}{\beta}\nabla^2 f(x^*) || + \frac{1}{2\beta} \int_0^1 || ty_k || dt  + \frac{1}{2\beta} \int_0^1 || t y_k - \frac{t}{\beta} \nabla f(x_k))  || dt \\
 & \leq  || I + \frac{1}{\beta}\nabla^2 f(x^*) || +  \frac{r_k}{4 \beta} + \frac{1}{2\beta} \int_0^1 || t y_k - \frac{t}{\beta} \nabla f(x_k))  || dt \\
 & \leq  || I + \frac{1}{\beta}\nabla^2 f(x^*) || +  \frac{r_k}{4 \beta} + \frac{1}{2\beta} \int_0^1 t || y_k - \frac{1}{\beta} \nabla f(x_k))  || dt \\
 & \leq  || I + \frac{1}{\beta}\nabla^2 f(x^*) || +  \frac{r_k}{4 \beta} + \frac{1}{2\beta} \int_0^1 || t y_k || dt   \\
 & \leq  || I + \frac{1}{\beta}\nabla^2 f(x^*) || +  \frac{r_k}{2 \beta} \\
 & \leq \frac{1}{\beta}  \lambda_{\max}(\nabla^2 f) + 1 + \frac{r_k}{4\beta}
\end{aligned}
\end{equation}

Using, the above inequalities we get:
\begin{equation}
\begin{aligned}
y_{k+1} &= H_k y_k + G_k \\
r_{k+1} & \leq  ||H_k|| r_k + ||G_k|| \\
& \leq \big(\frac{1}{\beta} \lambda_{\max}(\nabla^2 f) + \frac{3}{2} \big)r_k + \frac{r_k^2}{4\beta} \\
r_{k+1} & \leq \mu_1 r_k + \mu_2 r_k^2
\end{aligned}
\end{equation}
